driver/Compiler.v
@@ -102,7 +102,7 @@ Require Rustlightgen.
 Require RustIRgen.
 Require InitAnalysis.
 Require ElaborateDrop.
-Require BorrowCheckPolonius.
+(* Require BorrowCheckPolonius. *)
 Require Clightgen.
 
 (** Proof of Rust frontend  *)
@@ -216,11 +216,11 @@ Definition transf_rust_program (p: Rustsyntax.program) : res Asm.program :=
   @@@ time "Rustsyntax to Rustlight" Rustlightgen.transl_program
   !@@ time "Rustlight to RustIR" RustIRgen.transl_program
   @@@ time "Elaborate drop in RustIR" ElaborateDrop.transl_program
-  @@@ time "Replace origins in RustIR" ReplaceOrigins.transl_program
-  @@@ time "Borrow check" (fun p => match BorrowCheckPolonius.borrow_check_program p with
-                                 | OK _ => OK p
-                                 | Error msg => Error msg
-                                 end)
+  (* @@@ time "Replace origins in RustIR" ReplaceOrigins.transl_program *)
+  (* @@@ time "Borrow check" (fun p => match BorrowCheckPolonius.borrow_check_program p with *)
+  (*                                | OK _ => OK p *)
+  (*                                | Error msg => Error msg *)
+  (*                                end) *)
   @@@ time "Generate Clight and insert drop glue" Clightgen.transl_program
   @@@ transf_clight_program.
 
