rustfrontend/RustIRsem.v
@@ -313,29 +313,30 @@ Inductive step : state -> trace -> state -> Prop :=
     step (Callstate vf vargs k m) t (Returnstate v k m')
    
 (** Return cases *)
-| step_return_0: forall e lb m1 m2 f k,
-    (forall id b t, e ! id = Some (b, t) -> complete_type ge t = true) ->
-    blocks_of_env ge e = lb ->
-    (* drop the stack blocks *)
-    Mem.free_list m1 lb = Some m2 ->
-    (* return unit or Vundef? *)
-    step (State f (Sreturn None) k e m1) E0 (Returnstate Vundef (call_cont k) m2)
-| step_return_1: forall le a v v1 lb m1 m2 f k,
-    eval_expr ge le m1 a v ->
+(* | step_return_0: forall e lb m1 m2 f k, *)
+(*     (forall id b t, e ! id = Some (b, t) -> complete_type ge t = true) -> *)
+(*     blocks_of_env ge e = lb -> *)
+(*     (* drop the stack blocks *) *)
+(*     Mem.free_list m1 lb = Some m2 -> *)
+(*     (* return unit or Vundef? *) *)
+(*     step (State f (Sreturn None) k e m1) E0 (Returnstate Vundef (call_cont k) m2) *)
+| step_return_1: forall le p v v1 lb m1 m2 f k,
+    eval_expr ge le m1 (Epure (Eplace p (typeof_place p))) v ->
+    (** TODO: reconsider this condition and check it in Clightgen *)
     (forall id b t, le ! id = Some (b, t) -> complete_type ge t = true) ->
     (* sem_cast to the return type *)
-    sem_cast v (typeof a) f.(fn_return) = Some v1 ->
+    sem_cast v (typeof_place p) f.(fn_return) = Some v1 ->
     (* drop the stack blocks *)
     blocks_of_env ge le = lb ->
     Mem.free_list m1 lb = Some m2 ->
-    step (State f (Sreturn (Some a)) k le m1) E0 (Returnstate v1 (call_cont k) m2)
+    step (State f (Sreturn p) k le m1) E0 (Returnstate v1 (call_cont k) m2)
 (* no return statement but reach the end of the function *)
-| step_skip_call: forall e lb m1 m2 f k,
-    is_call_cont k ->
-    (forall id b t, e ! id = Some (b, t) -> complete_type ge t = true) ->
-    blocks_of_env ge e = lb ->
-    Mem.free_list m1 lb = Some m2 ->
-    step (State f Sskip k e m1) E0 (Returnstate Vundef (call_cont k) m2)
+(* | step_skip_call: forall e lb m1 m2 f k, *)
+(*     is_call_cont k -> *)
+(*     (forall id b t, e ! id = Some (b, t) -> complete_type ge t = true) -> *)
+(*     blocks_of_env ge e = lb -> *)
+(*     Mem.free_list m1 lb = Some m2 -> *)
+(*     step (State f Sskip k e m1) E0 (Returnstate Vundef (call_cont k) m2) *)
          
 | step_returnstate: forall p v b ofs m1 m2 e f k,
     eval_place ge e m1 p b ofs ->
@@ -563,16 +564,16 @@ Inductive step_mem_error : state -> Prop :=
     (FIND: Genv.find_funct ge vf = Some (Internal f)),
     function_entry_mem_error f vargs m e ->
     step_mem_error (Callstate vf vargs k m)
-| step_return_0_error: forall f k le m,
+(* | step_return_0_error: forall f k le m, *)
+(*     Mem.free_list m (blocks_of_env ge le) = None -> *)
+(*     step_mem_error (State f (Sreturn None) k le m) *)
+| step_return_1_error1: forall f p k le m,
+    eval_expr_mem_error ge le m (Epure (Eplace p (typeof_place p))) ->
+    step_mem_error (State f (Sreturn p) k le m)
+| step_return_2_error2: forall f p k le m v,
+    eval_expr ge le m (Epure (Eplace p (typeof_place p))) v ->
     Mem.free_list m (blocks_of_env ge le) = None ->
-    step_mem_error (State f (Sreturn None) k le m)
-| step_return_1_error1: forall f a k le m,
-    eval_expr_mem_error ge le m a ->
-    step_mem_error (State f (Sreturn (Some a)) k le m)
-| step_return_2_error2: forall f a k le m v,
-    eval_expr ge le m a v ->
-    Mem.free_list m (blocks_of_env ge le) = None ->
-    step_mem_error (State f (Sreturn (Some a)) k le m)
+    step_mem_error (State f (Sreturn p) k le m)
 | step_skip_call_error: forall f k le m,
     is_call_cont k ->
     Mem.free_list m (blocks_of_env ge le) = None ->
